messageInvariantPrototypes/ringLeaderElection/automate/spec.dfy
@@ -6,21 +6,21 @@ module Obligations {
   import opened DistributedSystem
 
 ghost predicate IsLeader(c: Constants, h: Hosts, idx: nat) 
-    requires h.WF(c)
-    requires c.ValidIdx(idx)
+  requires h.WF(c)
+  requires c.ValidIdx(idx)
 {
-    h.hosts[idx].highestHeard == c.hostConstants[idx].hostId
+  h.hosts[idx].highestHeard == c.hostConstants[idx].hostId
 }
 
 ghost predicate Safety(c: Constants, v: Variables) 
-    requires v.WF(c)
+  requires v.WF(c)
 {
-    forall idx1, idx2 | 
-        && c.ValidIdx(idx1) 
-        && c.ValidIdx(idx2) 
-        && IsLeader(c, v.Last(), idx1)
-        && IsLeader(c, v.Last(), idx2)
-        :: idx1 == idx2
+  forall idx1, idx2 | 
+    && c.ValidIdx(idx1) 
+    && c.ValidIdx(idx2) 
+    && IsLeader(c, v.Last(), idx1)
+    && IsLeader(c, v.Last(), idx2)
+    :: idx1 == idx2
 }
 }
 
